extracted_code/TestEquality.ml
@@ -7,6 +7,13 @@ let get_program f =
   close_in x;
   str |> Sexp.of_string |> CrTypeIF.coq_CaracaraProgram_of_sexp
 
+let get_general_program f =
+  let x = open_in f in
+  let len = in_channel_length x in
+  let str = really_input_string x len in
+  close_in x;
+  str |> Sexp.of_string |> CrTypeIF.CrModule.coq_GeneralCaracaraProgram_of_sexp
+
 let get_mem_program f = MemSolver.load_program f
 
 let print_equiv = function
@@ -178,3 +185,10 @@ let%expect_test "e2e bpf test: O0 ≡ O2" =
     running query...
     Z3Unsat
     |}]
+
+(* Test 13: linear scan vs tss for simple filter database *)
+let%expect_test "tss basic" =
+  let p1 = get_general_program "../test/lin_pkt.out" in
+  let p2 = get_general_program "../test/tss_pkt.out" in
+  print_equiv (SmtModuleQuery.modnet_equivalence_checker p1 p2);
+  [%expect {| Equivalent |}]
