SmtExpr.v
@@ -114,5 +114,3 @@ with eval_smt_mem (e : SmtArrExpr) (v : SmtValuation) : Memory CrVal :=
     | SmtArrInit => @CrVal.tabula_rasa CrVal
     | SmtArrSt e1 e2 e3 e4 => CrVal.st (eval_smt_mem e1 v) ((*eval_smt_ptr*) eval_smt_arith e2 v) (eval_smt_arith e3 v) (eval_smt_arith e4 v)
     end.
-
-(* InitStatus: might be unnecessary and error prone because Z3 may not map 1-to-1 to this. *)
